Make UniversalAlgebra multisorted.

Numbers.v
@@ -1,5 +1,4 @@
-Require RingCat.
-Require Import Structures CatStuff RingOps FieldOps.
+Require Import Structures CatStuff RingOps FieldOps SemiRingAlgebra RingAlgebra.
 
 Class Naturals A {e plus mult zero one} :=
   { naturals_ring:> SemiRing e plus mult zero one
@@ -17,16 +16,16 @@ Section nicer_naturals_initial.
   Definition naturals_to_semiring_arrow: semiring.Arrow (semiring.as_object N) (semiring.as_object SR)
      := proj1_sig (naturals_initial (semiring.as_object SR)).
 
-  Definition naturals_to_semiring: N -> SR := proj1_sig naturals_to_semiring_arrow.
+  Definition naturals_to_semiring: N -> SR := proj1_sig naturals_to_semiring_arrow tt.
 
-  Lemma naturals_to_semring_unique (f: N -> SR) (h: SemiRing_Morphism f): forall x, f x == naturals_to_semiring x.
+  Lemma naturals_to_semiring_unique (f: N -> SR) (h: SemiRing_Morphism f): forall x, f x == naturals_to_semiring x.
   Proof.
    unfold naturals_to_semiring, naturals_to_semiring_arrow.
    destruct (naturals_initial), x.
    unfold semiring.Arrow, UniversalAlgebra.Arrow in e1.
    simpl in *. intros. symmetry.
-   apply (((fun p => e1 (exist _ f p) x0: x x0 == f x0))).
-   constructor. apply _.
+   apply (((fun p => e1 (exist (UA.HomoMorphism semiring.sig (fun _ : unit => N) (fun _ : unit => SR)) (fun _ => f) p) tt x0: x tt x0 == f x0))).
+   constructor. intro. apply _.
    destruct o; simpl.
       apply preserves_plus.
      apply preserves_mult.
@@ -37,9 +36,13 @@ Section nicer_naturals_initial.
   Definition naturals_to_semiring_mor: SemiRing_Morphism naturals_to_semiring.
   Proof.
    unfold naturals_to_semiring.
-   intros.
    destruct naturals_to_semiring_arrow.
-   apply (@hmok _ _ _ _ semiring.impl_from_instance semiring.impl_from_instance _ _ _ _).
+   simpl.
+   simpl in h.
+   apply (@semiring.morphism_from_ua N _ (fun _ => SR) (fun _ => equiv) semiring.impl_from_instance semiring.impl_from_instance x h _ H0 tt).
+(*
+   Check (@semiring.morphism_from_ua N _ (fun _ => SR) (fun _ => equiv) semiring.impl_from_instance semiring.impl_from_instance _ _ _ H0).
+*)
   Qed. (* making this an instance causes weird ring problems. see ringbug.v *)
 
 End nicer_naturals_initial.
@@ -51,17 +54,50 @@ Proof.
  generalize (@naturals_initial B _ _ _ _ _ _), (@naturals_initial A _ _ _ _ _ _).
  intros.
  destruct (@initials_unique semiring.Object semiring.Arrow _ _ _ _ _ (semiring.as_object A) (semiring.as_object B) i0 i).
- apply (H2 a).
+ apply (H2 tt a).
 Qed.
 
 Class Integers A {e plus mult opp zero one} :=
   { integers_ring:> Ring e plus mult opp zero one
-  ; integers_initial: @initial RingCat.O RingCat.A RingCat.a_equiv (RingCat.MkO A)
+  ; integers_initial: @initial _ ring.Arrow _ (ring.as_object A)
   ; integers_eqdec:> Decidable e }.
 
-Definition integers_to_ring `{Integers In} `{Ring R}: In -> R := proj1_sig (proj1_sig (integers_initial (RingCat.MkO R))).
+Section nicer_integers_initial.
+
+  Context `{Integers Int} R `{Ring R}.
+
+  Definition integers_to_ring_arrow: ring.Arrow (ring.as_object Int) (ring.as_object R)
+     := proj1_sig (integers_initial (ring.as_object R)).
+
+  Definition integers_to_ring: Int -> R := proj1_sig integers_to_ring_arrow tt.
+
+  Lemma integers_to_ring_unique (f: Int -> R) (h: Ring_Morphism f): forall x, f x == integers_to_ring x.
+  Proof.
+   unfold integers_to_ring, integers_to_ring_arrow.
+   destruct (integers_initial), x.
+   unfold semiring.Arrow, UniversalAlgebra.Arrow in e1.
+   simpl in *. intros. symmetry.
+   apply (((fun p => e1 (exist (UA.HomoMorphism ring.sig (fun _ : unit => Int) (fun _ : unit => R)) (fun _ => f) p) tt x0: x tt x0 == f x0))).
+   constructor. intro. apply _.
+   destruct o; simpl.
+       apply preserves_plus.
+      apply preserves_mult.
+     apply preserves_0.
+    apply preserves_1.
+   apply preserves_inv.
+  Qed.
+
+  Definition integers_to_ring_mor: Ring_Morphism integers_to_ring.
+  Proof.
+   unfold integers_to_ring.
+   destruct integers_to_ring_arrow.
+   simpl in h.
+   apply (@ring.morphism_from_ua Int _ (fun _ => R) (fun _ => equiv) ring.impl_from_instance ring.impl_from_instance x h _ H0 tt).
+  Qed.
+
+End nicer_integers_initial.
 
 Class Rationals A {e plus mult opp zero one mult_inv leq} :=
   { rationals_ordfield:> OrdField e plus mult opp zero one mult_inv leq
   ; rationals_eqdec:> Decidable e
-  ; rationals_frac: forall `{i: Integers B} (t := integers_to_ring) (a: A), exists num: B, exists den: B, a == t num * / t den }.
+  ; rationals_frac: forall `{i: Integers B} (t := integers_to_ring A) (a: A), exists num: B, exists den: B, a == t num * / t den }.
