RingAlgebra.v
@@ -8,30 +8,47 @@ Section contents.
 
   Inductive op := plus | mult | zero | one | opp.
 
-  Definition sig: UA.Signature := UA.Build_Signature op
-    (fun o => match o with plus => 2 | mult => 2 | zero => 0 | one => 0 | opp => 1 end)%nat.
+  Section sig.
+    Import UA.op_type_notations.
+
+  Let sorts := unit.
+
+  Definition sig: UA.Signature := UA.Build_Signature op sorts
+    (fun o => match o with
+      | plus => tt -=> tt -=> UA.constant _ tt
+      | mult => tt -=> tt -=> UA.constant _ tt
+      | zero => UA.constant _ tt
+      | one => UA.constant _ tt
+      | opp => tt -=> UA.constant _ tt
+      end)%nat.
+
+  End sig.
 
   Section impl.
 
     Context `{Ring A}.
 
-    Definition impl_from_instance: UA.Implementation sig A := fun o =>
+    Definition impl_from_instance: UA.Implementation sig (fun _ => A) := fun o =>
       match o with plus => ring_plus | mult => ring_mult | zero => 0 | one => 1 | opp => group_inv end.
 
-    Global Instance: @UA.Propers sig A _ impl_from_instance.
+    Global Instance: @UA.Propers sig (fun _ => A) (fun _ => equiv) impl_from_instance.
     Proof. intro o. destruct o; simpl; try apply _; unfold Proper; reflexivity. Qed.
 
   End impl.
 
-  Global Instance: RingPlus (UA.Term sig 0) := fun x => UA.App sig _ (UA.App sig _ (UA.Op sig plus) x).
-  Global Instance: RingMult (UA.Term sig 0) := fun x => UA.App sig _ (UA.App sig _ (UA.Op sig mult) x).
-  Global Instance: GroupInv (UA.Term sig 0) := UA.App sig _ (UA.Op sig opp).
-  Global Instance: RingZero (UA.Term sig 0) := UA.Op sig zero.
-  Global Instance: RingOne (UA.Term sig 0) := UA.Op sig one.
+  Global Instance: RingPlus (UA.Term sig (UA.constant _ tt)) :=
+    fun x => UA.App sig _ _ (UA.App sig _ _ (UA.Op sig plus) x).
+  Global Instance: RingMult (UA.Term sig (UA.constant _ tt)) :=
+    fun x => UA.App sig _ _ (UA.App sig _ _ (UA.Op sig mult) x).
+  Global Instance: RingZero (UA.Term sig (UA.constant _ tt)) := UA.Op sig zero.
+  Global Instance: RingOne (UA.Term sig (UA.constant _ tt)) := UA.Op sig one.
+  Global Instance: GroupInv (UA.Term sig (UA.constant _ tt)) := UA.App sig _ _ (UA.Op sig opp).
 
-  Local Notation x := (UA.Var sig 0).
-  Local Notation y := (UA.Var sig 1).
-  Local Notation z := (UA.Var sig 2).
+  Local Notation x := (UA.Var sig 0 tt).
+  Local Notation y := (UA.Var sig 1 tt).
+  Local Notation z := (UA.Var sig 2 tt).
+
+  Import UA.notations.
 
   Inductive E: UA.Statement sig -> Prop :=
     |e_plus_assoc: E (x + (y + z) === (x + y) + z)
@@ -42,8 +59,9 @@ Section contents.
     |e_mult_1_l: E (1 * x === x)
     |e_mult_0_l: E (0 * x === 0)
     |e_distr: E (x * (y + z) === x * y + x * z)
-    |.
+    |e_plus_opp: E (x + - x === 0).
 
+(*
   Definition e_distr_r `{e: Equiv A} `{!Equivalence e} `{UA.Implementation sig A} `{@UA.Propers sig A _ _}:
     (forall e: UA.Statement sig, E e -> (forall v, UA.eval_stmt sig A v e)) -> forall vars, UA.eval_stmt sig A vars ((x + y) * z === x * z + y * z).
   Proof.
@@ -56,80 +74,121 @@ Section contents.
     apply (H1 _ e_mult_comm (fun v => match v: nat with 0 => vars 2%nat | _ => vars 0%nat end)).
    apply (H1 _ e_mult_comm (fun v => match v: nat with 0 => vars 2%nat | _ => vars 1%nat end)).
   Qed.
+*)
 
-  Lemma laws_from_semiring `{SemiRing}: forall e, E e -> forall vars, @UA.eval_stmt sig A _ impl_from_instance vars e.
+  Lemma laws_from_instance `{Ring}: forall e, E e ->
+    forall vars, @UA.eval_stmt sig (fun _ => A) (fun _ => equiv) impl_from_instance vars e.
   Proof.
    intros.
    inversion_clear H0; simpl.
-          apply associativity.
-         apply commutativity.
-        apply plus_0_l.
-       apply associativity.
-      apply commutativity.
-     apply mult_1_l.
-    apply mult_0_l.
-   apply distribute_l.
+           apply associativity.
+          apply commutativity.
+         apply plus_0_l.
+        apply associativity.
+       apply commutativity.
+      apply mult_1_l.
+     apply mult_0_l.
+    apply distribute_l.
+   apply plus_opp_r.
   Qed.
 
   Definition Object := UA.Variety sig E.
   Definition Arrow := UA.Arrow sig E.
 
-  Definition as_object A `{SemiRing A}: Object := @UA.MkVariety sig E A _ _ _ _ laws_from_semiring.
+  Definition as_object A `{Ring A}: Object.
+   set (impl_from_instance).
+   apply (@UA.MkVariety sig E (fun _ => A) (fun _ => equiv) i _).
+    apply _.
+   apply (@laws_from_instance A), _.
+  Defined.
 
-  Section ring_ops_from_semiring_homo.
+  Section ops_from_impl.
+
     Context `{UA.Implementation sig A}.
-    Global Instance: RingPlus A := UA.op sig plus.
-    Global Instance: RingMult A := UA.op sig mult.
-    Global Instance: RingZero A := UA.op sig zero.
-    Global Instance: RingOne A := UA.op sig one.
 
-  Definition instance_from_impl `{e: Equiv A} `{!Equivalence e} `{!UA.Propers sig A}
-    (variety_laws: forall e, E e -> forall vars, @UA.eval_stmt sig A _ _ vars e): @SemiRing A _ _ _ _ _. (* todo: tweak implicits such that the underscores aren't needed here *)
-  Proof with auto.
-   repeat (constructor; try apply _); repeat intro.
-               apply (variety_laws _ e_mult_assoc (fun n => match n with 0 => x | 1 => y | _ => z end)).
-              apply (@UA.propers sig A _ _ _ mult)...
-             apply (variety_laws _ e_mult_1_l (fun n => x)).
-            rewrite_with (variety_laws _ e_mult_comm (fun n => match n with 0 => x | _ => mon_unit end)).
-            apply (variety_laws _ e_mult_1_l (fun n => x)).
-           apply (variety_laws _ e_plus_assoc (fun n => match n with 0 => x | 1 => y | _ => z end)).
-          apply (@UA.propers sig A _ _ _ plus)...
-         apply (variety_laws _ e_plus_0_l (fun n => x)).
-        rewrite_with (variety_laws _ e_plus_comm (fun n => match n with 0 => x | _ => RingZero_instance_1 end)).
-        apply (variety_laws _ e_plus_0_l (fun n => x)).
-       apply (variety_laws _ e_plus_comm (fun n => match n with 0 => x | _ => y end)).
-      apply (variety_laws _ e_mult_comm (fun n => match n with 0 => x | _ => y end)).
-     apply (variety_laws _ e_distr (fun n => match n with 0 => a | 1 => b | _ => c end)).
-    apply (@e_distr_r _ _ _ _ _ variety_laws (fun n => match n with 0 => a | 1 => b | _ => c end)).
-   apply (variety_laws _ e_mult_0_l (fun n => x)).
-  Qed.
+    Global Instance: RingPlus (A tt) := UA.op sig plus.
+    Global Instance: RingMult (A tt) := UA.op sig mult.
+    Global Instance: RingZero (A tt) := UA.op sig zero.
+    Global Instance: RingOne (A tt) := UA.op sig one.
+    Global Instance: GroupInv (A tt) := UA.op sig opp.
 
-  End ring_ops_from_semiring_homo.
+    Definition instance_from_impl `{e: forall s, Equiv (A s)} `{!forall s, Equivalence (e s)} `{!UA.Propers sig A}
+      (variety_laws: forall e, E e -> forall vars, @UA.eval_stmt sig A _ _ vars e): @Ring (A tt) _ _ _ _ _ _.
+    Proof with auto.
+     repeat (constructor; try apply _); repeat intro.
+                   apply (variety_laws _ e_plus_assoc (fun s n => match s with tt => match n with 0 => x | 1 => y | _ => z end end)).
+                  apply (@UA.propers sig A _ _ _ plus)...
+                 apply (variety_laws _ e_plus_0_l (fun s n => match s with tt => x end)).
+                pose proof (variety_laws _ e_plus_comm (fun s n => match s with tt => match n with 0 => x | _ => RingZero_instance_1 end end)).
+                simpl in H2. rewrite H2.
+                apply (variety_laws _ e_plus_0_l (fun s n => match s with tt => x end)).
+               apply (@UA.propers sig A _ _ _ opp)...
+              admit.
+             apply (variety_laws _ e_plus_opp (fun s n => match s with tt => x end)).
+            apply (variety_laws _ e_plus_comm (fun s n => match s with tt => match n with 0 => x | _ => y end end)).
+           apply (variety_laws _ e_mult_assoc (fun s n => match s with tt => match n with 0 => x | 1 => y | _ => z end end)).
+          apply (@UA.propers sig A _ _ _ mult)...
+         apply (variety_laws _ e_mult_1_l (fun s n => match s with tt => x end)).
+        pose proof (variety_laws _ e_mult_comm (fun s n => match s with tt => match n with 0 => x | _ => mon_unit end end)).
+        simpl in H2. rewrite H2.
+        apply (variety_laws _ e_mult_1_l (fun s n => match s with tt => x end)).
+       apply (variety_laws _ e_mult_comm (fun s n => match s with tt => match n with 0 => x | _ => y end end)).
+      apply (variety_laws _ e_distr (fun s n => match s with tt => match n with 0 => a | 1 => b | _ => c end end)).
+     admit. (* todo *)
+      (*apply (@e_distr_r _ _ _ _ _ variety_laws (fun n => match n with 0 => a | 1 => b | _ => c end)).*)
+    Qed.
 
-  Definition Variety_as_SemiRing (o: Object): @SemiRing o _ _ _ _ _.
+  End ops_from_impl.
+
+  Definition from_object (o: Object): @Ring (o tt) _ _ _ _ _ _.
   Proof. apply (instance_from_impl (UA.variety_laws _ _ o)). Qed.
     (* not an instance because we don't want this to be used accidentally *)
 
+  Section morphism_from_ua.
+
+    Context  `{e0: Equiv R0} {R1: unit -> Type} `{e1: forall u, Equiv (R1 u)} `{!Equivalence e0}
+      `{forall u, Equivalence (e1 u)}
+      `{UA.Implementation sig (fun _ => R0)} `{UA.Implementation sig R1}
+      (f: forall u, R0 -> R1 u)
+        `{!@UA.HomoMorphism sig (fun _ => R0) R1 (fun _ => e0) e1 _ _ f}.
+
+    Global Instance: RingPlus R0 := @UA.op sig (fun _ => R0) _ plus.
+    Global Instance: RingMult R0 := @UA.op sig (fun _ => R0) _ mult.
+    Global Instance: RingZero R0 := @UA.op sig (fun _ => R0) _ zero.
+    Global Instance: RingOne R0 := @UA.op sig (fun _ => R0) _ one.
+    Global Instance: GroupInv R0 := @UA.op sig (fun _ => R0) _ opp.
+
+    Global Instance: RingPlus (R1 u) := match u with tt => @UA.op sig R1 _ plus end.
+    Global Instance: RingMult (R1 u) := match u with tt => @UA.op sig R1 _ mult end.
+    Global Instance: RingZero (R1 u) := match u with tt => @UA.op sig R1 _ zero end.
+    Global Instance: RingOne (R1 u) := match u with tt => @UA.op sig R1 _ one end.
+    Global Instance: GroupInv (R1 u) := match u with tt => @UA.op sig R1 _ opp end.
+
+    Definition morphism_from_ua (sr0: @Ring R0 _ _ _ _ _ _) (sr1: @Ring (R1 tt) _ _ _ _ _ _):
+     forall u, Ring_Morphism (f u).
+    Proof.
+     destruct u.
+     pose proof (@UA.preserves sig (fun _ => _) R1 (fun _ => e0) e1 _ _ f _).
+     repeat (constructor; try apply _).
+           apply (@UA.homo_proper sig (fun _ => _) _ (fun _ => _) _ _ _ f _).
+          apply (H3 plus).
+         apply (H3 zero).
+        apply (H3 opp).
+       apply (@UA.homo_proper sig (fun _ => _) _ (fun _ => _) _ _ _ f _).
+      apply (H3 mult).
+     apply (H3 one).
+    Qed.
+
+(*
+    Definition homo_preserves_plus: forall a b, f (a + b) == f a + f b.  Proof UA.preserves sig f plus.
+    Definition homo_preserves_mult: forall a b, f (a * b) == f a * f b.  Proof UA.preserves sig f mult.
+    Definition homo_preserves_0: f 0 == 0.  Proof UA.preserves sig f zero.
+    Definition homo_preserves_1: f 1 == 1.  Proof UA.preserves sig f one.
+*)
+      (* these should go, eventually *)
+
+  End morphism_from_ua.
+
 End contents.
-End semiring.
 
-Section soup.
-
-  Context  `{e0: Equiv R0} `{e1: Equiv R1} `{!Equivalence e0} `{!Equivalence e1}
-    `{UA.Implementation semiring.sig R0} `{UA.Implementation semiring.sig R1}
-    (f: R0 -> R1) `{!UA.HomoMorphism semiring.sig f}.
-
-  Definition hmok (sr0: @SemiRing R0 _ _ _ _ _) (sr1: @SemiRing R1 _ _ _ _ _): SemiRing_Morphism f.
-   repeat (constructor; try apply _).
-      apply (UA.preserves semiring.sig f semiring.plus).
-     apply (UA.preserves semiring.sig f semiring.zero).
-    apply (UA.preserves semiring.sig f semiring.mult).
-   apply (UA.preserves semiring.sig f semiring.one).
-  Qed.
-
-  Definition homo_preserves_plus: forall a b, f (a + b) == f a + f b.  Proof UA.preserves semiring.sig f semiring.plus.
-  Definition homo_preserves_mult: forall a b, f (a * b) == f a * f b.  Proof UA.preserves semiring.sig f semiring.mult.
-  Definition homo_preserves_0: f 0 == 0.  Proof UA.preserves semiring.sig f semiring.zero.
-  Definition homo_preserves_1: f 1 == 1.  Proof UA.preserves semiring.sig f semiring.one.
-
-End soup.
+End ring.
