UniversalAlgebra.v
@@ -1,84 +1,123 @@
-
 Require Import
   Morphisms Setoid List CanonicalNames CatStuff Program.
 
-Inductive Signature: Type := { sign_op:> Set; arity:> sign_op -> nat }.
+Section pointwise_dependent_relation. Context A (B: A -> Type) (R: forall a, relation (B a)).
 
-(* op_type translates arities into operation types (e.g. 2 is mapped to A->A->A). *)
+  Definition pointwise_dependent_relation: relation (forall a, B a) :=
+    fun f f' => forall a, R _ (f a) (f' a).
 
-Fixpoint op_type A (n: nat): Type :=
-  match n with
-  | 0 => A
-  | S n' => A -> op_type A n'
-  end.
+  Global Instance pdr_equiv `{forall a, Equivalence (R a)}: Equivalence pointwise_dependent_relation.
+  Proof. firstorder. Qed.
 
-(* Extensional equality for operations of arbitrary arity: *)
+End pointwise_dependent_relation. (* todo: move elsewhere *)
 
-Definition op_type_equiv `{e: Equiv A}: forall n, Equiv (op_type A n) :=
- fix F (n: nat) :=
-  match n return Equiv (op_type A n) with
-  | 0 => equiv
-  | S n' => (equiv ==> F n')%signature
-  end.
+Section with_atomic. Variable Atomic: Set.
 
-Existing Instance op_type_equiv.
+  Inductive OpType: Set :=
+    | constant (a: Atomic)
+    | function (a: Atomic) (g: OpType).
 
-(* op_type_equiv is /almost/ an equivalence relation. Note that is is /not/ readily reflexive. *)
-
-Instance sig_type_trans `{e: Equiv A} `{!Reflexive e} `{!Transitive e}: Transitive (op_type_equiv n).
-Proof. induction n. assumption. simpl. intros x y z. unfold equiv, respectful. eauto. Qed.
-
-Instance sig_type_sym `{e: Equiv A} `{!Symmetric e}: Symmetric (op_type_equiv n).
-Proof with try assumption. induction n... simpl. intro. unfold respectful. symmetry. apply H. symmetry... Qed.
-
-(* Given maps between A and B, there are maps between op_type A and op_type B: *)
-
-Section map_op.
-
-  Context {A B: Type} `{!Equiv A} `{!Equiv B} (f: A -> B) (g: B -> A)
-    `{!Proper (equiv ==> equiv) f} `{!Proper (equiv ==> equiv) g}.
-
-  Fixpoint map_op {n: nat}: op_type A n -> op_type B n :=
-      match n return op_type A n -> op_type B n with
-      | 0 => fun x => f x
-      | S n' => fun x => fun y => map_op (x (g y))
+  Definition op_type (T: Atomic -> Type): OpType -> Type :=
+    fix F (t: OpType): Type :=
+      match t with
+      | constant a => T a
+      | function a g => T a -> F g
       end.
 
-  Global Instance map_op_proper: Proper (equiv ==> equiv) (@map_op n).
-  Proof.
-   induction n; simpl; repeat intro. firstorder.
-   apply IHn, (H (g x0) (g y0)). firstorder.
-  Qed.
+  Section with_atomic_inter. Variable T: Atomic -> Type.
 
-End map_op.
+    Definition op_type_equiv
+       `{e: forall A, Equiv (T A)}: forall o: OpType, Equiv (op_type T o) :=
+     fix F (o: OpType): Equiv (op_type T o) :=
+      match o return Equiv (op_type T o) with
+      | constant A => e A
+      | function A g => (e A ==> F g)%signature
+      end.
+
+    Existing Instance op_type_equiv.
+
+    (* op_type_equiv is /almost/ an equivalence relation. Note that is is /not/ readily reflexive. *)
+
+    Global Instance sig_type_trans `{e: forall A, Equiv (T A)} `{forall A, Reflexive (e A)} `{forall A, Transitive (e A)}: Transitive (op_type_equiv o).
+    Proof. induction o; simpl; firstorder. Qed.
+
+    Global Instance sig_type_sym `{e: forall A, Equiv (T A)} `{forall A, Symmetric (e A)}: Symmetric (op_type_equiv o).
+    Proof. induction o; simpl; firstorder. Qed.
+
+    Lemma sig_type_refl `{e: forall A, Equiv (T A)} `{forall a, Reflexive (e a)} (o: OpType) a (x: op_type T (function a o)) y:
+      Proper equiv x ->
+      op_type_equiv o (x y) (x y).
+    Proof.
+     intros.
+     apply (H0 y y).
+     reflexivity.
+    Qed.
+
+  End with_atomic_inter.
+
+  Existing Instance op_type_equiv.
+
+  Section map_op.
+
+    (* Given maps between two sets of atomics, there are maps between the corresponding op_types*)
+
+    Context {A B: Atomic -> Type} `{forall a, Equiv (A a)} `{forall a, Equiv (B a)}
+     (ab: forall a, A a -> B a) (ba: forall a, B a -> A a)
+     `{forall a, Proper (equiv ==> equiv) (ab a)}
+     `{forall a, Proper (equiv ==> equiv) (ba a)}.
+
+    Fixpoint map_op {o: OpType}: op_type A o -> op_type B o :=
+      match o return op_type A o -> op_type B o with
+      | constant u => ab u
+      | function u v => fun x => fun y => map_op (x (ba u y))
+      end.
+
+    Global Instance map_op_proper o: Proper (op_type_equiv A o ==> op_type_equiv B o) (@map_op o).
+    Proof. induction o; simpl; firstorder. Qed.
+
+  End map_op.
+
+End with_atomic.
+
+Inductive Signature: Type :=
+  { sign_op:> Set
+  ; sign_atomics: Set
+  ; sign_sig:> sign_op -> OpType sign_atomics }.
 
 Section for_signature. Variable sign: Signature.
 
-  Class Implementation A := op: forall o, op_type A (sign o).
+  Class Implementation (A: sign_atomics sign -> Type) := op: forall o, op_type _ A (sign o).
 
-  Class Propers A `{Equiv A} `{Implementation A} := propers:> forall o: sign, Proper (op_type_equiv (sign o)) (op o).
+  Class Propers (A: sign_atomics sign -> Type) `{forall a, Equiv (A a)} `{Implementation A} :=
+    propers:> forall o: sign, Proper (op_type_equiv _ A (sign o)) (op o).
 
-  Inductive Term: nat -> Set :=
-    | Var (v: nat): Term 0
-    | App n: Term (S n) -> Term 0 -> Term n
+  Inductive Term: OpType (sign_atomics sign) -> Set :=
+    | Var (v: nat) (a: sign_atomics sign): Term (constant _ a)
+    | App (t: OpType (sign_atomics sign)) y:  Term (function _ y t) -> Term (constant _ y) -> Term t
     | Op (o: sign): Term (sign o).
 
-  Inductive Statement: Type := Eq (a b: Term 0) | Impl (a b: Statement) | Ext (P: Prop).
+  Inductive Statement: Type := Eq t (a b: Term (constant _ t)) | Impl (a b: Statement) | Ext (P: Prop).
 
-  Section for_map. Context `{ea: Equiv A} `{eb: Equiv B} `{Implementation A} `{Implementation B} (f: A -> B).
+  Section for_map.
+    Context (A: sign_atomics sign -> Type) (B: sign_atomics sign -> Type)
+      `{ea: forall a, Equiv (A a)} `{eb: forall a, Equiv (B a)}
+      `{!Implementation A} `{!Implementation B} (f: forall a, A a -> B a).
 
-    Fixpoint Preservation {n: nat}: op_type A n -> op_type B n -> Prop :=
-      match n return op_type A n -> op_type B n -> Prop with
-      | 0 => fun o o' => f o == o'
-      | S n' => fun o o' => forall x, Preservation (o x) (o' (f x))
+    Implicit Arguments f [[a]].
+
+    Fixpoint Preservation {n: OpType (sign_atomics sign)}: op_type _ A n -> op_type _ B n -> Prop :=
+      match n return op_type _ A n -> op_type _ B n -> Prop with
+      | constant d => fun o o' => f o == o'
+      | function x y => fun o o' => forall x, Preservation (o x) (o' (f x))
       end.
 
     Class HomoMorphism: Prop :=
-      { homo_proper:> Proper (equiv ==> equiv) f
+      { homo_proper:> forall a, Proper (equiv ==> equiv) (@f a)
       ; preserves: forall (o: sign), Preservation (op o) (op o) }.
 
-    Instance Preservation_proper `{HomoMorphism} `{!Equivalence ea} `{!Equivalence eb} n:
-      Proper (op_type_equiv n ==> op_type_equiv n ==> iff) (@Preservation n).
+    Global Instance Preservation_proper `{HomoMorphism}
+      `{!forall a, Equivalence (ea a)} `{!forall a, Equivalence (eb a)} n:
+      Proper (op_type_equiv _ A n ==> op_type_equiv _ B n ==> iff) (@Preservation n).
     Proof.
      induction n.
       repeat intro.
@@ -86,40 +125,61 @@ Section for_signature. Variable sign: Signature.
        rewrite <- H2, <- H3. assumption.
       rewrite H2, H3. assumption.
      repeat intro.
-     split; repeat intro; simpl;
+     split; simpl; repeat intro;
       apply (IHn (x x1) (y x1) (H2 x1 x1 (reflexivity _)) (x0 (f x1)) (y0 (f x1)) (H3 (f x1) (f x1) (reflexivity _)));
       apply (H4 x1).
     Qed.
 
   End for_map.
 
-  Section eval. Context A `{ea: Equiv A} `{!Equivalence ea} `{!Implementation A} `{!Propers A}.
+  Section Vars.
 
-    Fixpoint eval {n: nat} (vars: nat -> A) (t: Term n) {struct t}: op_type A n :=
-      match t in Term n return op_type A n with
-      | Var v => vars v
+    Context (A: sign_atomics sign -> Type) `{e: forall a, Equiv (A a)} `{forall a, Equivalence (e a)}.
+
+    Definition Vars := forall a, nat -> A a.
+
+    Global Instance: Equiv Vars :=
+     @pointwise_dependent_relation (sign_atomics sign) (fun a => nat -> A a)
+      (fun _ => pointwise_relation _ equiv).
+
+    Global Instance: Equivalence (equiv: relation Vars).
+
+  End Vars.
+
+  Section eval.
+
+    Context 
+     `{ea: forall a, Equiv (A a)} `{!forall a, Equivalence (ea a)} `{!Implementation A} `{@Propers A ea _}.
+
+    Fixpoint eval {n: OpType (sign_atomics sign)} (vars: Vars A) (t: Term n) {struct t}:
+        op_type _ A n :=
+      match t in Term n return op_type _ A n with
+      | Var v a => vars a v
       | Op o => op o
-      | App n f a => eval vars f (eval vars a)
+      | App n a f p => eval vars f (eval vars p)
       end.
 
-    Global Instance eval_proper (n: nat): Proper (pointwise_relation _ equiv ==> eq ==> equiv) (@eval n).
+    Let bla := op_type_equiv (sign_atomics sign) A.
+
+    Global Instance eval_proper (n: OpType (sign_atomics sign)):
+      Proper (equiv ==> eq ==> equiv) (@eval n).
     Proof with auto.
      do 7 intro. subst.
      induction y0.
-       apply H...
+       apply H1...
       apply IHy0_1...
      apply propers.
     Qed.
 
-    Definition eval_stmt (vars: nat -> A): Statement -> Prop :=
+    Definition eval_stmt (vars: Vars A): Statement -> Prop :=
       fix F (s: Statement) :=
       match s with
-      | Eq a b => eval vars a == eval vars b
+      | Eq _ a b => eval vars a == eval vars b
       | Impl a b => F a -> F b
       | Ext P => P
       end.
 
-    Global Instance eval_stmt_proper: Proper (pointwise_relation _ equiv ==> eq ==> iff) eval_stmt.
+    Global Instance eval_stmt_proper: Proper (equiv ==> eq ==> iff) eval_stmt.
     Proof with auto.
      intros v v' ve s s' se. subst.
      induction s'; simpl.
@@ -135,12 +195,13 @@ Section for_signature. Variable sign: Signature.
   Section category. Variable E: Statement -> Prop.
 
     Record Variety: Type := MkVariety
-      { variety_carrier:> Type
-      ; variety_equiv: Equiv variety_carrier
-      ; variety_op:> Implementation variety_carrier
-      ; variety_equivalence: Equivalence variety_equiv
-      ; variety_propers: Propers variety_carrier
-      ; variety_laws: forall s, E s -> forall vars, eval_stmt _ vars s
+      { variety_atomics:> sign_atomics sign -> Type
+      ; variety_equiv: forall a, Equiv (variety_atomics a)
+      ; variety_op:> Implementation variety_atomics
+      ; variety_equivalence: forall a, Equivalence (variety_equiv a)
+      ; variety_propers: Propers variety_atomics
+      ; variety_laws: forall s, E s -> forall vars: forall a, nat -> variety_atomics a,
+          @eval_stmt variety_atomics variety_equiv variety_op vars s
      }.
 
     Existing Instance variety_equivalence.
@@ -148,33 +209,39 @@ Section for_signature. Variable sign: Signature.
     Existing Instance variety_propers.
     Existing Instance variety_equiv.
 
-    Definition Arrow (X Y: Variety): Type := sig (@HomoMorphism X _ Y _ _ _).
+    Definition Arrow (X Y: Variety): Type := sig (@HomoMorphism X Y _ _ _ _).
 
-    Global Program Instance: CatId Variety Arrow := fun o => id.
+    Global Program Instance: CatId Variety Arrow := fun _ _ => id.
 
     Next Obligation.
-     constructor. apply _.
-     unfold id.
-     intro.
-     generalize (@op o _ o0). intro.
-     induction (sign o0); simpl; intuition.
+     constructor. intro. apply _.
+     unfold id. intro.
+     generalize (@op (variety_atomics H) (variety_op H) o). intro.
+     induction (sign_sig sign o); simpl; intuition.
     Qed.
 
-    Global Program Instance: CatComp Variety Arrow := fun x y z => fun f g v => (`f) ((`g) v).
+    Global Program Instance: CatComp Variety Arrow := fun x y z => fun f g v a => (`f) _ ((`g) v a).
 
     Next Obligation. Proof with reflexivity.
      destruct f. destruct g.
-     constructor. repeat intro. simpl. rewrite H...
+     constructor. repeat intro. simpl.
+      pose proof (@homo_proper x y _ _ _ _ x1 _ a).
+      pose proof (@homo_proper y z _ _ _ _ x0 _ a).
+      rewrite H...
      intros. simpl.
-     generalize (preserves x1 o) (preserves x0 o).
+     generalize (preserves _ _ x1 o) (preserves _ _ x0 o).
      generalize (@op z _ o) (@op y _ o) (@op x _ o).
-     induction (sign o); simpl; intros. rewrite H. assumption.
-     apply (IHn (o0 (x0 (x1 x2))) (o1 (x1 x2))); auto.
+     induction (sign o); simpl; intros. 
+      pose proof (@homo_proper x y _ _ _ _ x1 _ a).
+      pose proof (@homo_proper y z _ _ _ _ x0 _ a).
+      rewrite H. assumption.
+     apply (@IHo0 (o1 (x0 _ (x1 _ x2))) (o2 (x1 _ x2))); auto.
     Qed.
 
     Global Instance o_equiv: Equiv Variety := eq.
 
-    Global Instance a_equiv (x y: Variety): Equiv (Arrow x y) := fun a a' => pointwise_relation _ equiv (proj1_sig a) (proj1_sig a').
+    Global Instance a_equiv (x y: Variety): Equiv (Arrow x y)
+      := fun a a' => forall b, pointwise_relation _ equiv (proj1_sig a b) (proj1_sig a' b).
 
     Global Instance homo_cat: Category Variety Arrow.
     Proof with auto.
@@ -185,7 +252,10 @@ Section for_signature. Variable sign: Signature.
          constructor; repeat intro.
            reflexivity.
           symmetry...
-         transitivity ((proj1_sig y) a)...
+          apply H.
+         transitivity ((proj1_sig y) b a)...
+          apply H.
+         apply H0.
         repeat intro.
         unfold equiv in *.
         unfold a_equiv in *.
@@ -196,93 +266,129 @@ Section for_signature. Variable sign: Signature.
         simpl in *.
         unfold pointwise_relation in *.
         intros.
+        pose proof (@homo_proper _ _ _ _ _ _ x _ b).
         rewrite H0.
         apply H.
        intros.
        destruct w. destruct y. destruct z. destruct x. intro. reflexivity.
-      intros. destruct x. destruct y. intro. reflexivity.
-     intros. destruct x. destruct y. intro. reflexivity.
+      intros. destruct x. destruct y. intro. intro. reflexivity.
+     intros. destruct x. destruct y. intro. intro. reflexivity.
     Qed.
 
   End category.
 
   Section for_isomorphic_implementations.
 
-    Context A B `{ea: Equiv A} `{eb: Equiv B} `{!Equivalence ea} `{!Equivalence eb} `{Implementation A} `{Implementation B}
+    Context (A B: sign_atomics sign -> Type)
+      `{ea: forall a, Equiv (A a)}
+      `{eb: forall a, Equiv (B a)}
+      `{forall a, Equivalence (ea a)} `{forall a, Equivalence (eb a)} `{Implementation A} `{Implementation B}
       `{!Propers A} `{!Propers B}
-      (ab: A->B) (ba: B->A)
-      `(@HomoMorphism _ _ _ _ _ _ ab) `(@HomoMorphism _ _ _ _ _ _ ba)
-      (iso_l: forall x, ba (ab x) == x) (iso_r: forall x, ab (ba x) == x).
+      (ab: forall a, A a -> B a) (ba: forall a, B a -> A a)
+      `(@HomoMorphism A B ea eb _ _ ab) `(@HomoMorphism _ _ _ _ _ _ ba)
+      (iso_l: forall a x, ba a (ab a x) == x) (iso_r: forall a x, ab a (ba a x) == x).
 
-    Lemma iso_vars_l (v: nat -> A): pointwise_relation _ equiv v (fun i => ba (ab (v i))).
+    Implicit Arguments ab [[a]].
+    Implicit Arguments ba [[a]].
+
+      (* Let us help out poor old instance resolution a bit: *)
+    Let ab_proper := homo_proper A B (@ab).
+    Let ba_proper:= homo_proper B A (@ba).
+    Let eval_proper_a := @eval_proper A ea H1 Propers0.
+    Let eval_proper_b := @eval_proper B eb H2 Propers1.
+
+    Lemma iso_vars_l (v: Vars A): v == (fun _ i => ba (ab (v _ i))).
     Proof. repeat intro. rewrite iso_l. reflexivity. Qed.
 
-    Lemma iso_vars_r (v: nat -> B): pointwise_relation _ equiv v (fun i => ab (ba (v i))).
+    Lemma iso_vars_r (v: Vars B): v == (fun _ i => ab (ba (v _ i))).
     Proof. repeat intro. rewrite iso_r. reflexivity. Qed.
 
     (* Evaluating a term in one implementation is "the same" as evaluating it in the other. *)
 
-    Lemma carry_eval n (t: Term n) (v: nat -> B): eval _ (fun i => ba (v i)) t == map_op ba ab (eval _ v t).
+    Instance blaya o: Equiv (op_type (sign_atomics sign) A o) :=
+      op_type_equiv (sign_atomics sign) A o.
+    Instance blaya' o: Equiv (op_type (sign_atomics sign) B o) :=
+      op_type_equiv (sign_atomics sign) B o.
+
+    Instance: Transitive (blaya o).
+    Proof. intro. apply _. Qed. (* this really shouldn't be necessary *)
+
+    Lemma carry_eval n (t: Term n) (v: Vars B): 
+      @eval A _ _ (fun _ i => ba (v _ i)) t == map_op _ (@ba) (@ab) (eval v t).
     Proof with auto.
      induction t; simpl in *; intros.
        reflexivity.
-      set (y := eval B v t2).
-      assert (eval B v t1 y == eval B v t1 (ab (ba y))).
-       clearbody y.
-       assert (y == ab (ba y)). symmetry. apply iso_r.
-       assert (pointwise_relation nat equiv v v). intro. reflexivity.
-       apply (eval_proper B (Datatypes.S n) v v H4)...
-      assert (map_op ba ab (eval B v t1 y) == map_op ba ab (eval B v t1 (ab (ba y)))).
-       apply (@map_op_proper B A _ _ ba ab _ _ n)...
-      transitivity (map_op ba ab (eval B v t1 (ab (ba y))))...
-       apply IHt1.
-       subst y.
-       apply IHt2.
-      symmetry...
+      set (eval (fun (a : sign_atomics sign) (i : nat) => ba (v a i)) t2).
+      pose proof (@eval_proper A ea H1 Propers0 (function (sign_atomics sign) y t1) (fun a i => ba (v a i))
+        (fun a i => ba (v a i)) (reflexivity _) t2 t2 (reflexivity _): 
+          Proper (ea y ==> op_type_equiv (sign_atomics sign) A t1)%signature o).
+      rewrite (IHt2 v).
+      subst o.
+      pose proof (IHt1 v (ba (eval v t3)) (ba (eval v t3))).
+      simpl in H6.
+      rewrite H6.
+       set (homo_proper A B (@ab)).
+       set (homo_proper B A (@ba)).
+       set (@map_op_proper (sign_atomics sign) B A _ _ (@ba) (@ab) p0 p).
+       unfold equiv.
+       apply (@map_op_proper (sign_atomics sign) B A _ _ (@ba) (@ab))...
+       pose proof (@eval_proper B eb H2 Propers1 _ v v (reflexivity _) t2 t2 (reflexivity _): Proper equiv (eval v t2)).
+       rewrite (iso_r _ (eval v t3)).
+       apply sig_type_refl...
+       intro. apply _.
+      reflexivity.
      pose proof (@propers A _ _ _ o).
      pose proof (@propers B _ _ _ o).
-     pose proof (@preserves A _ B _ _ _ ab _ o).
-     revert H3 H4 H5.
+     pose proof (@preserves A B _ _ _ _ (@ab) _ o).
+     revert H5 H6 H7.
      clear v.
-     generalize (@op A H o) (@op B H0 o).
+     generalize (@op A H1 o) (@op B H2 o).
      induction (sign o).
       simpl.
       intros.
-      rewrite <- iso_l. rewrite H5. reflexivity.
+      rewrite <- iso_l.
+      pose proof (@homo_proper B A _ _ _ _ (@ba) _ a (ab o0) o1).
+      apply H8 in H7.
+      assumption. (* weird *)
      simpl.
+     unfold Proper. unfold respectful.
      repeat intro.
-     apply IHn.
-       apply H3. reflexivity.
-      apply H4. reflexivity.
-     assert (ab x == ab y). rewrite H6. reflexivity.
-     apply (Preservation_proper ab _ _ _ (H3 x x (reflexivity _)) _ _ (H4 (ab x) (ab y) H7)).
-     apply H5.
+     unfold blaya.
+     apply IHo0.
+       apply H5. reflexivity.
+      apply H6. reflexivity.
+     assert (op_type_equiv (sign_atomics sign) A o0 (o1 x) (o1 y)).
+      apply H5. assumption.
+     apply (@Preservation_proper A B ea eb H1 H2 (@ab) H3 _ _ o0 (o1 x) (o1 y) H9 (o2 (ab y)) (o2 (ab y)))...
+     change (o2 (ab y) == o2 (ab y)).
+     apply H6.
+     reflexivity.
     Qed. (* todo: clean up *)
 
     (* Similarly, evaluating a statement in one implementation is "the same" as evaluating it in the other. *)
 
-    Lemma carry_stmt_with (s: Statement) (v: nat -> A):
-      eval_stmt A v s <-> eval_stmt B (fun i => ab (v i)) s.
+    Lemma carry_stmt_with (s: Statement) (v: Vars A):
+      eval_stmt v s <-> @eval_stmt B _ _ (fun _ i => ab (v _ i)) s.
     Proof with auto.
      intros.
      induction s; simpl.
        split; intros.
-        rewrite <- (iso_r (eval B (fun i => ab (v i)) a)).
-        rewrite <- (iso_r (eval B (fun i => ab (v i)) b)).
-        rewrite <- (carry_eval 0 a (fun i => ab (v i))).
-        rewrite <- (carry_eval 0 b (fun i => ab (v i))).
+        rewrite <- (iso_r _ (eval (fun a0 i => ab (v a0 i)) a)).
+        rewrite <- (iso_r _ (eval (fun a0 i => ab (v a0 i)) b)).
+        rewrite <- (carry_eval _ a (fun d i => ab (v d i))).
+        rewrite <- (carry_eval _ b (fun d i => ab (v d i))).
         rewrite <- iso_vars_l.
-        rewrite H3.
+        rewrite H5.
         reflexivity.
        rewrite iso_vars_l.
        do 2 rewrite carry_eval.
-       simpl. rewrite H3. reflexivity.
+       simpl. rewrite H5. reflexivity.
       firstorder.
      intuition.
     Qed.
 
-    Lemma carry_stmt (s: Statement): (forall v, eval_stmt A v s) -> (forall v, eval_stmt B v s).
-    Proof. intros. rewrite iso_vars_r. rewrite <- carry_stmt_with. apply H3. Qed.
+    Lemma carry_stmt (s: Statement): (forall v, @eval_stmt A _ _ v s) -> (forall v, @eval_stmt B _ _ v s).
+    Proof. intros. rewrite iso_vars_r. rewrite <- carry_stmt_with. apply H5. Qed.
 
   End for_isomorphic_implementations.
 
@@ -293,7 +399,11 @@ Existing Instance variety_equivalence.
 Existing Instance variety_equiv.
 Existing Instance variety_propers.
 
+Module op_type_notations.
+  Global Infix "-=>" := (function _) (at level 95, right associativity).
+End op_type_notations.
+
 Module notations.
-  Global Infix "===" := (Eq _) (at level 70, no associativity).
+  Global Infix "===" := (Eq _ _) (at level 70, no associativity).
   Global Infix "-=>" := (Impl _) (at level 95, right associativity).
 End notations.
